Graphiti/Core/Rewrites/JoinComm.lean
@@ -13,27 +13,26 @@ namespace Graphiti.JoinComm
 
 open StringModule
 
-def identMatcher (s : String) (g : ExprHigh String String) : RewriteResult (List String × List String) := do
-  let n ← ofOption (.error s!"{decl_name%}: could not find '{s}'") <| g.modules.find? s
-  unless "join".isPrefixOf n.2 do throw (.error s!"{decl_name%}: type of '{s}' is '{n.2}' instead of 'join'")
+variable (T : Vector Nat 1)
+variable (M : Nat)
 
-  let (.some t1) := n.2.splitOn[1]? | throw (.error s!"{decl_name%}: type incorrect1")
-  let (.some t2) := n.2.splitOn[2]? | throw (.error s!"{decl_name%}: type incorrect2")
+def identMatcher (s : String) : Pattern String (String × Nat) 1 := fun g => do
+  let n ← ofOption' (.error s!"{decl_name%}: could not find '{s}'") <| g.modules.find? s
+  unless "join" == n.2.1 do throw (.error s!"{decl_name%}: type of '{s}' is '{n.2}' instead of 'join'")
+  return ([s], #v[n.2.2])
 
-  return ([s], [t1, t2])
-
-def matcher (g : ExprHigh String String) : RewriteResult (List String × List String) :=
+def matcher : Pattern String (String × Nat) 1 := fun g => do
   throw (.error s!"{decl_name%}: matcher not implemented")
 
 def identRenaming (s : String) (g : ExprHigh String String) : RewriteResult (AssocList String (Option String)) := do
   return (.cons s "joinN" .nil)
 
-def lhs (T₁ T₂ : Type) (S₁ S₂ : String) : ExprHigh String String × IdentMap String (TModule1 String) := [graphEnv|
+def lhs : ExprHigh String (String × Nat) := [graph|
     i_0 [type = "io"];
     i_1 [type = "io"];
     o_out [type = "io"];
 
-    join [typeImp = $(⟨_, join T₁ T₂⟩), type = $(s!"join {S₁} {S₂}")];
+    join [type = "join", arg = $(T[0])];
 
     i_0 -> join [to = "in1"];
     i_1 -> join [to = "in2"];
@@ -41,20 +40,17 @@ def lhs (T₁ T₂ : Type) (S₁ S₂ : String) : ExprHigh String String × Iden
     join -> o_out [from = "out1"];
   ]
 
-def lhs_extract S₁ S₂ := (lhs Unit Unit S₁ S₂).fst.extract ["join"] |>.get rfl
+def lhs_extract := (lhs T).extract ["join"] |>.get rfl
+theorem double_check_empty_snd : (lhs_extract T).snd = ExprHigh.mk ∅ ∅ := by rfl
+def lhsLower := (lhs_extract T).fst.lower.get rfl
 
-theorem double_check_empty_snd S₁ S₂ : (lhs_extract S₁ S₂).snd = ExprHigh.mk ∅ ∅ := by rfl
-
-def lhsLower S₁ S₂ := (lhs_extract S₁ S₂).fst.lower.get rfl
-
-def rhs (T₁ T₂ : Type) (S₁ S₂ : String) : ExprHigh String String × IdentMap String (TModule1 String) := [graphEnv|
+def rhs : ExprHigh String (String × Nat) := [graph|
     i_0 [type = "io"];
     i_1 [type = "io"];
     o_out [type = "io"];
 
-    joinN [typeImp = $(⟨_, join T₂ T₁⟩), type = $(s!"join {S₂} {S₁}")];
-    pure [typeImp = $(⟨_, @StringModule.pure (T₂ × T₁) (T₁ × T₂) (λ (a, b) => (b, a))⟩),
-          type = $(s!"pure ({S₂}×{S₁}) ({S₁}×{S₂})")];
+    joinN [type = "join", arg = $(M+1)];
+    pure [type = "pure", arg = $(M+2)];
 
     i_0 -> joinN [to = "in2"];
     i_1 -> joinN [to = "in1"];
@@ -64,22 +60,21 @@ def rhs (T₁ T₂ : Type) (S₁ S₂ : String) : ExprHigh String String × Iden
     pure -> o_out [from = "out1"];
   ]
 
-def rhs_extract S₁ S₂ := (rhs Unit Unit S₁ S₂).fst.extract ["joinN", "pure"] |>.get rfl
+def rhs_extract := (rhs M).extract ["joinN", "pure"] |>.get rfl
+def rhsLower := (rhs_extract M).fst.lower.get rfl
+def findRhs mod := (rhs_extract 0).fst.modules.find? mod |>.map Prod.fst
 
-def rhsLower S₁ S₂ := (rhs_extract S₁ S₂).fst.lower.get rfl
-
-def findRhs mod := (rhs_extract "" "").fst.modules.find? mod |>.map Prod.fst
-
-def rewrite : Rewrite String String :=
-  { abstractions := [],
-    pattern := matcher,
-    rewrite := λ | [S₁, S₂] => pure ⟨lhsLower S₁ S₂, rhsLower S₁ S₂⟩ | _ => failure,
+def rewrite : Rewrite String (String × Nat) :=
+  { abstractions := []
+    params := 1
+    pattern := matcher
+    rewrite := λ l n => ⟨lhsLower l, rhsLower n⟩
     name := "join-comm"
     transformedNodes := [findRhs "joinN" |>.get rfl]
     addedNodes := [findRhs "pure" |>.get rfl]
+    fresh_types := 2
   }
 
-def targetedRewrite (s : String) : Rewrite String String :=
-  { rewrite with pattern := identMatcher s }
+def targetedRewrite s := { rewrite with pattern := identMatcher s }
 
 end Graphiti.JoinComm
