Graphiti/Core/Rewrites/PureRewrites.lean
@@ -20,164 +20,147 @@ open StringModule
 
 namespace Constant
 
-def extract_type (typ : String) : RewriteResult (List String) := do
-  let [typName, num] := typ.splitOn | throw .done
-  unless typName = "constant" do throw .done
-  return [num]
+def extract_type (typ : String × Nat) : RewriteResultSL (Vector Nat 1) := do
+  unless typ.1 == "constant" do throw .done
+  return #v[typ.2]
 
 def match_node := Graphiti.match_node extract_type
 
-def matcher (g : ExprHigh String String) : RewriteResult (List String × List String) :=
+def matcher : Pattern String (String × Nat) 1 := fun g => do
   throw (.error s!"{decl_name%}: matcher not implemented")
 
-variable (n : Nat)
+variable (T : Vector Nat 1)
+variable (M : Nat)
 
-def lhs : ExprHigh String String × IdentMap String (TModule1 String) := [graphEnv|
+def lhs : ExprHigh String (String × Nat) := [graph|
     i [type = "io"];
     o [type = "io"];
 
-    const [typeImp = $(⟨_, constant n⟩), type = $(s!"constant {n}")];
+    const [type = "constant", arg = $(T[0])];
 
     i -> const [to="in1"];
     const -> o [from="out1"];
   ]
 
-def lhs_extract := (lhs n).fst.extract ["const"] |>.get rfl
+def lhs_extract := (lhs T).extract ["const"] |>.get rfl
+theorem double_check_empty_snd : (lhs_extract T).snd = ExprHigh.mk ∅ ∅ := by rfl
+def lhsLower := (lhs_extract T).fst.lower.get rfl
 
-theorem double_check_empty_snd : (lhs_extract n).snd = ExprHigh.mk ∅ ∅ := by rfl
-
-def lhsLower := lhs_extract n |>.fst.lower.get rfl
-
-def rhs : ExprHigh String String × IdentMap String (TModule1 String) := [graphEnv|
+def rhs : ExprHigh String (String × Nat) := [graph|
     i [type = "io"];
     o [type = "io"];
 
-    const [typeImp = $(⟨_, pure (S := Unit) λ _ => n⟩), type = $(s!"pure Unit T")];
+    const [type = "pure", arg = $(M+1)];
 
     i -> const [to="in1"];
     const -> o [from="out1"];
   ]
 
-def findRhs mod := (rhs 0).1.modules.find? mod |>.map Prod.fst
+def rhsLower := (rhs M).lower.get rfl
+def findRhs mod := (rhs 0).modules.find? mod |>.map Prod.fst
 
-def rhsLower := (rhs n).fst.lower.get rfl
-
-def rewrite : Rewrite String String :=
-  { abstractions := [],
-    pattern := matcher,
-    rewrite := λ l => do
-      let n' ← l[0]?
-      -- SOMEDAY: Replace this by a proper Nat parser
-      let exp ← Lean.Json.Parser.num.run n' |>.toOption
-      let parsed ← exp.mantissa.toNat'
-      return ⟨ lhsLower parsed, rhsLower parsed ⟩
-    name := .some "pure-constant"
-    transformedNodes := [findRhs "const" |>.get rfl]
-  }
+def rewrite : Rewrite String (String × Nat) where
+  abstractions := []
+  params := 1
+  pattern := matcher
+  rewrite := λ l n => ⟨lhsLower l, rhsLower n⟩
+  name := .some "pure-constant"
+  transformedNodes := [findRhs "const" |>.get rfl]
+  fresh_types := 1
 
 end Constant
 
 namespace Operator1
 
-def extract_type (typ : String) : RewriteResult (List String) := do
-  let [typName, typ1, typ2, op] := typ.splitOn | throw .done
-  unless typName = "operator1" do throw .done
-  return [typ1, typ2, op]
+def extract_type (typ : String × Nat) : RewriteResultSL (Vector Nat 1) := do
+  unless typ.1 == "operator1" do throw .done
+  return #v[typ.2]
 
 def match_node := Graphiti.match_node extract_type
 
-def matcher (g : ExprHigh String String) : RewriteResult (List String × List String) :=
+def matcher : Pattern String (String × Nat) 1 := fun g => do
   throw (.error s!"{decl_name%}: not implemented")
 
-variable (T₁ T : Type)
-variable [Inhabited T]
-variable (T₁ₛ Tₛ Op : String)
+variable (T : Vector Nat 1)
+variable (M : Nat)
 
-def lhs : ExprHigh String String × IdentMap String (TModule1 String) := [graphEnv|
+def lhs : ExprHigh String (String × Nat) := [graph|
     i [type = "io"];
     o [type = "io"];
 
-    op [typeImp = $(⟨_, operator1 T₁ T Op⟩), type = $(s!"operator1 {T₁ₛ} {Tₛ} {Op}")];
+    op [type = "operator1", arg = $(T[0])];
 
     i -> op [to="in1"];
     op -> o [from="out1"];
   ]
 
-def lhs_extract := (lhs Unit Unit T₁ₛ Tₛ Op).fst.extract ["op"] |>.get rfl
+def lhs_extract := (lhs T).extract ["op"] |>.get rfl
+theorem double_check_empty_snd : (lhs_extract T).snd = ExprHigh.mk ∅ ∅ := by rfl
+def lhsLower := (lhs_extract T).fst.lower.get rfl
 
-theorem double_check_empty_snd : (lhs_extract T₁ₛ Tₛ Op).snd = ExprHigh.mk ∅ ∅ := by rfl
-
-def lhsLower := lhs_extract T₁ₛ Tₛ Op |>.fst.lower.get rfl
-
-def rhs : ExprHigh String String × IdentMap String (TModule1 String) := [graphEnv|
+def rhs : ExprHigh String (String × Nat) := [graph|
     i [type = "io"];
     o [type = "io"];
 
-    op [typeImp = $(⟨_, StringModule.pure λ x => @NatModule.op1_function T _ T₁ Op x⟩),
-        type = $(s!"pure {T₁ₛ} {Tₛ}")];
+    op [type = "pure", arg = $(M+1)];
 
     i -> op [to="in1"];
     op -> o [from="out1"];
   ]
 
-def findRhs mod := (rhs Unit Unit "" "" "").1.modules.find? mod |>.map Prod.fst
+def rhs_extract := (rhs M).extract ["op"] |>.get rfl
+def rhsLower := (rhs_extract M).fst.lower.get rfl
+def findRhs mod := (rhs_extract 0).fst.modules.find? mod |>.map Prod.fst
 
-def rhsLower := (rhs Unit Unit T₁ₛ Tₛ Op).fst.lower.get rfl
-
-def rewrite : Rewrite String String :=
+def rewrite : Rewrite String (String × Nat) :=
   { abstractions := [],
+    params := 1
     pattern := matcher,
-    rewrite :=
-      λ | [T1s, Ts, Ops] => .some ⟨ lhsLower T1s Ts Ops, rhsLower T1s Ts Ops ⟩
-        | _ => .none
+    rewrite := λ l n => ⟨lhsLower l, rhsLower n⟩
     name := .some "pure-operator1"
     transformedNodes := [findRhs "op" |>.get rfl]
+    fresh_types := 1
   }
 
 end Operator1
 
 namespace Operator2
 
-def extract_type (typ : String) : RewriteResult (List String) := do
-  let [typName, typ1, typ2, typ3, op] := typ.splitOn | throw .done
-  unless typName = "operator2" do throw .done
-  return [typ1, typ2, typ3, op]
+def extract_type (typ : String × Nat) : RewriteResultSL (Vector Nat 1) := do
+  unless typ.1 == "operator2" do throw .done
+  return #v[typ.2]
 
 def match_node := Graphiti.match_node extract_type
 
-def matcher (g : ExprHigh String String) : RewriteResult (List String × List String) :=
+variable (T : Vector Nat 1)
+variable (M : Nat)
+
+def matcher : Pattern String (String × Nat) 1 := fun g => do
   throw (.error s!"{decl_name%}: not implemented")
 
-variable (T₁ T₂ T : Type)
-variable [Inhabited T]
-variable (T₁ₛ T₂ₛ Tₛ Op : String)
-
-def lhs : ExprHigh String String × IdentMap String (TModule1 String) := [graphEnv|
+def lhs : ExprHigh String (String × Nat) := [graph|
     i1 [type = "io"];
     i2 [type = "io"];
     o [type = "io"];
 
-    op [typeImp = $(⟨_, operator2 T₁ T₂ T Op⟩), type = $(s!"operator2 {T₁ₛ} {T₂ₛ} {Tₛ} {Op}")];
+    op [type = "operator2", arg = $(T[0])];
 
     i1 -> op [to="in1"];
     i2 -> op [to="in2"];
     op -> o [from="out1"];
   ]
 
-def lhs_extract := (lhs Unit Unit Unit T₁ₛ T₂ₛ Tₛ Op).fst.extract ["op"] |>.get rfl
+def lhs_extract := (lhs T).extract ["op"] |>.get rfl
+theorem double_check_empty_snd : (lhs_extract T).snd = ExprHigh.mk ∅ ∅ := by rfl
+def lhsLower := (lhs_extract T).fst.lower.get rfl
 
-theorem double_check_empty_snd : (lhs_extract T₁ₛ T₂ₛ Tₛ Op).snd = ExprHigh.mk ∅ ∅ := by rfl
-
-def lhsLower := lhs_extract T₁ₛ T₂ₛ Tₛ Op |>.fst.lower.get rfl
-
-def rhs : ExprHigh String String × IdentMap String (TModule1 String) := [graphEnv|
+def rhs : ExprHigh String (String × Nat) := [graph|
     i1 [type = "io"];
     i2 [type = "io"];
     o [type = "io"];
 
-    join [typeImp = $(⟨_, join T₁ T₂⟩), type = $(s!"join {T₁ₛ} {T₂ₛ}")];
-    op [typeImp = $(⟨_, StringModule.pure λ x => @NatModule.op2_function T _ T₁ T₂ Op x.1 x.2⟩),
-        type = $(s!"pure ({T₁ₛ}×{T₂ₛ}) {Tₛ}")];
+    join [type = "join", arg = $(M+1)];
+    op [type = "pure", arg = $(M+2)];
 
     i1 -> join [to="in1"];
     i2 -> join [to="in2"];
@@ -185,48 +168,44 @@ def rhs : ExprHigh String String × IdentMap String (TModule1 String) := [graphE
     op -> o [from="out1"];
   ]
 
-def rhs_extract := (rhs Unit Unit Unit T₁ₛ T₂ₛ Tₛ Op).fst.extract ["op", "join"] |>.get rfl
+def rhs_extract := (rhs M).extract ["op", "join"] |>.get rfl
+def rhsLower := (rhs_extract M).fst.lower.get rfl
+def findRhs mod := (rhs_extract 0).fst.modules.find? mod |>.map Prod.fst
 
-def findRhs mod := (rhs_extract "" "" "" "").1.modules.find? mod |>.map Prod.fst
-
-def rhsLower := (rhs_extract T₁ₛ T₂ₛ Tₛ Op).fst.lower.get rfl
-
-def rewrite : Rewrite String String :=
+def rewrite : Rewrite String (String × Nat) :=
   { abstractions := [],
+    params := 1
     pattern := matcher,
-    rewrite :=
-      λ | [T1s, T2s, Ts, Ops] => .some ⟨ lhsLower T1s T2s Ts Ops, rhsLower T1s T2s Ts Ops ⟩
-        | _ => .none
+    rewrite := λ l n => ⟨lhsLower l, rhsLower n⟩
     name := .some "pure-operator2"
     transformedNodes := [findRhs "op" |>.get rfl]
     addedNodes := [findRhs "join" |>.get rfl]
+    fresh_types := 2
   }
 
 end Operator2
 
 namespace Operator3
 
-def extract_type (typ : String) : RewriteResult (List String) := do
-  let [typName, typ1, typ2, typ3, typ4, op] := typ.splitOn | throw .done
-  unless typName = "operator3" do throw .done
-  return [typ1, typ2, typ3, typ4, op]
+def extract_type (typ : String × Nat) : RewriteResultSL (Vector Nat 1) := do
+  unless typ.1 == "operator3" do throw .done
+  return #v[typ.2]
 
 def match_node := Graphiti.match_node extract_type
 
-def matcher (g : ExprHigh String String) : RewriteResult (List String × List String) :=
+def matcher : Pattern String (String × Nat) 1 := fun g => do
   throw (.error s!"{decl_name%}: not implemented")
 
-variable (T₁ T₂ T₃ T : Type)
-variable [Inhabited T]
-variable (T₁ₛ T₂ₛ T₃ₛ Tₛ Op : String)
+variable (T : Vector Nat 1)
+variable (M : Nat)
 
-def lhs : ExprHigh String String × IdentMap String (TModule1 String) := [graphEnv|
+def lhs : ExprHigh String (String × Nat) := [graph|
     i1 [type = "io"];
     i2 [type = "io"];
     i3 [type = "io"];
     o [type = "io"];
 
-    op [typeImp = $(⟨_, operator3 T₁ T₂ T₃ T Op⟩), type = $(s!"operator3 {T₁ₛ} {T₂ₛ} {T₃ₛ} {Tₛ} {Op}")];
+    op [type = "operator3", arg = $(T[0])];
 
     i1 -> op [to="in1"];
     i2 -> op [to="in2"];
@@ -234,22 +213,19 @@ def lhs : ExprHigh String String × IdentMap String (TModule1 String) := [graphE
     op -> o [from="out1"];
   ]
 
-def lhs_extract := (lhs Unit Unit Unit Unit T₁ₛ T₂ₛ T₃ₛ Tₛ Op).fst.extract ["op"] |>.get rfl
+def lhs_extract := (lhs T).extract ["op"] |>.get rfl
+theorem double_check_empty_snd : (lhs_extract T).snd = ExprHigh.mk ∅ ∅ := by rfl
+def lhsLower := (lhs_extract T).fst.lower.get rfl
 
-theorem double_check_empty_snd : (lhs_extract T₁ₛ T₂ₛ T₃ₛ Tₛ Op).snd = ExprHigh.mk ∅ ∅ := by rfl
-
-def lhsLower := lhs_extract T₁ₛ T₂ₛ T₃ₛ Tₛ Op |>.fst.lower.get rfl
-
-def rhs : ExprHigh String String × IdentMap String (TModule1 String) := [graphEnv|
+def rhs : ExprHigh String (String × Nat) := [graph|
     i1 [type = "io"];
     i2 [type = "io"];
     i3 [type = "io"];
     o [type = "io"];
 
-    join1 [typeImp = $(⟨_, join T₂ T₃⟩), type = $(s!"join {T₂ₛ} {T₃ₛ}")];
-    join2 [typeImp = $(⟨_, join T₁ (T₂ × T₃)⟩), type = $(s!"join {T₁ₛ} ({T₂ₛ}×{T₃ₛ})")];
-    op [typeImp = $(⟨_, StringModule.pure λ (x : T₁ × T₂ × T₃) => @NatModule.op3_function T _ T₁ T₂ T₃ Op x.1 x.2.1 x.2.2⟩),
-        type = $(s!"pure ({T₁ₛ}×({T₂ₛ}×{T₃ₛ})) {Tₛ}")];
+    join1 [type = "join", arg = $(M+1)];
+    join2 [type = "join", arg = $(M+2)];
+    op [type = "pure", arg = $(M+3)];
 
     i1 -> join2 [to="in1"];
     i2 -> join1 [to="in1"];
@@ -261,68 +237,60 @@ def rhs : ExprHigh String String × IdentMap String (TModule1 String) := [graphE
     op -> o [from="out1"];
   ]
 
-def rhs_extract := (rhs Unit Unit Unit Unit T₁ₛ T₂ₛ T₃ₛ Tₛ Op).fst.extract ["op", "join1", "join2"] |>.get rfl
+def rhs_extract := (rhs M).extract ["op", "join1", "join2"] |>.get rfl
+def rhsLower := (rhs_extract M).fst.lower.get rfl
+def findRhs mod := (rhs_extract 0).fst.modules.find? mod |>.map Prod.fst
 
-def findRhs mod := (rhs_extract "" "" "" "" "").1.modules.find? mod |>.map Prod.fst
-
-def rhsLower := (rhs_extract T₁ₛ T₂ₛ T₃ₛ Tₛ Op).fst.lower.get rfl
-
-def rewrite : Rewrite String String :=
-  { abstractions := [],
-    pattern := matcher,
-    rewrite :=
-      λ | [T1s, T2s, T3s, Ts, Ops] => .some ⟨ lhsLower T1s T2s T3s Ts Ops, rhsLower T1s T2s T3s Ts Ops ⟩
-        | _ => .none
+def rewrite : Rewrite String (String × Nat) :=
+  { abstractions := []
+    params := 1
+    pattern := matcher
+    rewrite := λ l n => ⟨lhsLower l, rhsLower n⟩
     name := .some "pure-operator3"
     transformedNodes := [findRhs "op" |>.get rfl]
     addedNodes := [findRhs "join1" |>.get rfl, findRhs "join2" |>.get rfl]
+    fresh_types := 3
   }
 
 end Operator3
 
 namespace Fork
 
-def extract_type (typ : String) : RewriteResult (List String) := do
-  let [typName, typ, num] := typ.splitOn | throw .done
-  unless typName = "fork" do throw .done
-  unless num = "2" do throw .done
-  return [typ]
+def extract_type (typ : String × Nat) : RewriteResultSL (Vector Nat 1) := do
+  unless typ.1 == "fork2" do throw .done
+  return #v[typ.2]
 
 def match_node := Graphiti.match_node extract_type
 
-def matcher (g : ExprHigh String String) : RewriteResult (List String × List String) :=
+def matcher : Pattern String (String × Nat) 1 := fun g => do
   throw (.error s!"{decl_name%}: not implemented")
 
-variable (T : Type)
-variable [Inhabited T]
-variable (Tₛ : String)
+variable (T : Vector Nat 1)
+variable (M : Nat)
 
-def lhs : ExprHigh String String × IdentMap String (TModule1 String) := [graphEnv|
+def lhs : ExprHigh String (String × Nat) := [graph|
     i [type = "io"];
     o1 [type = "io"];
     o2 [type = "io"];
 
-    fork [typeImp = $(⟨_, fork T 2⟩), type = $(s!"fork {Tₛ} 2")];
+    fork [type = "fork2", arg = $(T[0])];
 
     i -> fork [to="in1"];
     fork -> o1 [from="out1"];
     fork -> o2 [from="out2"];
   ]
 
-def lhs_extract := (lhs Unit Tₛ).fst.extract ["fork"] |>.get rfl
+def lhs_extract := (lhs T).extract ["fork"] |>.get rfl
+theorem double_check_empty_snd : (lhs_extract T).snd = ExprHigh.mk ∅ ∅ := by rfl
+def lhsLower := (lhs_extract T).fst.lower.get rfl
 
-theorem double_check_empty_snd : (lhs_extract Tₛ).snd = ExprHigh.mk ∅ ∅ := by rfl
-
-def lhsLower := lhs_extract Tₛ |>.fst.lower.get rfl
-
-def rhs : ExprHigh String String × IdentMap String (TModule1 String) := [graphEnv|
+def rhs : ExprHigh String (String × Nat) := [graph|
     i [type = "io"];
     o1 [type = "io"];
     o2 [type = "io"];
 
-    op [typeImp = $(⟨_, StringModule.pure λ (x : T) => (x, x)⟩),
-        type = $(s!"pure {Tₛ} ({Tₛ}×{Tₛ})")];
-    split [typeImp = $(⟨_, split T T⟩), type = $(s!"split {Tₛ} {Tₛ}")];
+    op [type = "pure", arg = $(M+1)];
+    split [type = "split", arg = $(M+2)];
 
     i -> op [to="in1"];
     op -> split [from="out1",to="in1"];
@@ -330,27 +298,25 @@ def rhs : ExprHigh String String × IdentMap String (TModule1 String) := [graphE
     split -> o2 [from="out2"];
   ]
 
-def rhs_extract := (rhs Unit Tₛ).fst.extract ["op", "split"] |>.get rfl
+def rhs_extract := (rhs M).extract ["op", "split"] |>.get rfl
+def rhsLower := (rhs_extract M).fst.lower.get rfl
+def findRhs mod := (rhs_extract 0).fst.modules.find? mod |>.map Prod.fst
 
-def rhsLower := (rhs_extract Tₛ).fst.lower.get rfl
-
-def findRhs mod := (rhs_extract "").1.modules.find? mod |>.map Prod.fst
-
-def rewrite : Rewrite String String :=
+def rewrite : Rewrite String (String × Nat) :=
   { abstractions := [],
+    params := 1
     pattern := matcher,
-    rewrite :=
-      λ | [Ts] => .some ⟨ lhsLower Ts, rhsLower Ts ⟩
-        | _ => .none
+    rewrite := λ l n => ⟨lhsLower l, rhsLower n⟩
     name := .some "pure-fork"
     transformedNodes := [.none]
     addedNodes := [findRhs "op" |>.get rfl, findRhs "split" |>.get rfl]
+    fresh_types := 2
   }
 
 end Fork
 
 -- TODO: do not pass the pattern, instead just precompute the pattern.
-def specialisedPureRewrites (p : Pattern String String) :=
+def specialisedPureRewrites (p : Pattern String (String × Nat) 1) :=
   [ { Constant.rewrite with
         pattern := fun g => do
           let (s :: _, t) ← p g | throw RewriteError.done
